ver2/eval_common.v
@@ -32,7 +32,7 @@ reverse order, the first in the list is the last update. *)
 Definition update_memory' (mem: memory) (update : memory_update EVMWord) :=
   match update with
   | U_MSTORE _ offset value => mstore mem offset value
-  | U_MSTORE8 _ offset value => mstore8 mem offset (split1 8 (EVMWordSize-8) value)
+  | U_MSTORE8 _ offset value => mstore mem (split1_byte (value: word ((S (pred BytesInEVMWord))*8))) offset 
   end.
 
 Fixpoint update_memory (mem: memory) (updates : memory_updates EVMWord) :=
